Gprog issue

verif/indices/verif_BtreeIndexASI.v
@@ -1,129 +1,308 @@
-Require Import btrees.relation_mem. (*needed for defining Vprog *)
+Require Import VST.floyd.VSU.
+Require Import VST.floyd.VSU_addmain.
 
 Require Import indices.spec_BtreeIndexASI.
-Require Import btrees.btrees_spec.
 Require Import indices.btree_instance.
 Require Import indices.btree_wrappers.
+
+Require Import btrees.relation_mem.
+Require Import btrees.btrees_spec.
 Require Import btrees.verif_newrel.
-(* Require Import btrees.verif_newcursor.
+Require Import btrees.verif_newcursor.
 Require Import btrees.verif_gotokey.
 Require Import btrees.verif_getrecord.
 Require Import btrees.verif_putrecord.
 Require Import btrees.verif_movetonext.
-Require Import btrees.verif_movetoprev. *)
+Require Import btrees.verif_movetoprev.
 
 Instance BtreeIndexCompSpecs : compspecs. make_compspecs prog. Defined.
 
-Require Import indices.Component.
-
 Section BtreeIndex_Component.
 
-  Definition BtreeIndexVprog : varspecs. mk_varspecs prog. Defined.
+Definition BtreeIndexVprog : varspecs. mk_varspecs prog. Defined.
 
-  Definition BI_ASI: funspecs := BtreeIndexASI.
+Definition BI_ASI: funspecs := BtreeIndexASI.
 
-  (*Definition conn_imported_specs := surely_malloc_specs.*)
+Definition spec_gprog: funspecs := btrees_spec.Gprog.
+Definition wrap_gprog: funspecs := btree_wrappers.Gprog.
 
-  Definition internal_specs: funspecs := BI_ASI.
+Definition internal_specs: funspecs := G_merge spec_gprog wrap_gprog.
 
-  Definition BtreeIndexGprog:funspecs := (*conn_imported_specs ++ *) internal_specs.
+Definition imported_specs := [currNode_spec].
 
-  Lemma cardinality_verif:
-    semax_body BtreeIndexVprog BtreeIndexGprog f_RL_NumRecords cardinality_funspec.
-  Proof.
-    eapply semax_body_funspec_sub. 
-    { replace BtreeIndexVprog with btrees_sep.Vprog by auto.
-      assert (K: BtreeIndexGprog = btree_wrappers.Gprog). admit. rewrite K.
-      apply body_NumRecords. } apply sub_cardinality.
-      simpl. repeat apply list_norepet_cons; auto.
-      unfold not. intros. inversion H. inversion H0. 
-      inversion H0. inversion H1. inversion H1.
-      unfold not. intros. inversion H. inversion H0. inversion H0.
-      apply list_norepet_nil.
-  Admitted.
+Definition BtreeIndexGprog:funspecs := (* imported_specs ++ *) internal_specs.
 
-  Lemma create_index_verif:
-    semax_body BtreeIndexVprog BtreeIndexGprog f_RL_NewRelation create_index_funspec.
-  Proof.
-    eapply semax_body_funspec_sub. 
-    { replace BtreeIndexVprog with btrees_sep.Vprog by auto.
-      assert (K: BtreeIndexGprog = btrees_spec.Gprog). admit. rewrite K.
-      apply body_NewRelation. } apply sub_create_index.
-      simpl. repeat apply list_norepet_cons; auto; 
-      try apply list_norepet_nil. 
-      unfold not. intros. inversion H. inversion H0. 
-      inversion H0. inversion H1. inversion H1. inversion H2. inversion H2.
-      unfold not. intros. inversion H. inversion H0. inversion H0. inversion H1.
-      inversion H1. unfold not. intros. inversion H. inversion H0. inversion H0.
-  Admitted.
-
-(*
-Lemma create_cursor_verif:
-    semax_body BtreeIndexVprog BtreeIndexGprog f_RL_NewCursor create_cursor_funspec.
+Lemma gprog_app_sub:  forall V G1 G2 f spec, 
+  list_norepet (map fst G2) -> 
+  list_norepet (map fst V ++ map fst (G1 ++ G2)) ->
+  semax_body V G2 f spec -> 
+  semax_body V (G1 ++ G2) f spec.
 Proof. 
+  intros. eapply semax_body_subsumption; eauto.
+  apply tycontext_sub_Gprog_app2; auto.
+Qed.
+
+Lemma gprog_gmerge_sub: forall V G1 G2 f spec, 
+  list_norepet (map fst G2) -> 
+  list_norepet (map fst V ++ map fst (G_merge G1 G2)) ->
+  semax_body V G2 f spec -> 
+  semax_body V (G_merge G1 G2) f spec.
+Proof. Admitted.
+
+
+Lemma list_norepet_spec_gprog: 
+  list_norepet (map fst spec_gprog).
+Proof. Admitted.
+
+Lemma list_norepet_vprog:
+  list_norepet (map fst BtreeIndexVprog).
+Proof. Admitted.
+
+
+Lemma list_norepet_wrap_gprog: 
+    list_norepet (map fst wrap_gprog).
+Proof. Admitted. 
+
+Lemma list_disjoint_vprog_gprog:
+  list_disjoint (map fst BtreeIndexVprog) (map fst (G_merge spec_gprog wrap_gprog)).
+Proof. Admitted.
+
+Lemma g_merge_comm: forall G1 G2, 
+  G_merge G1 G2 = G_merge G2 G1.
+Proof. Admitted.
+
+Lemma gprog_wrap_sub: forall f s,
+  semax_body BtreeIndexVprog wrap_gprog f s ->
+  semax_body BtreeIndexVprog BtreeIndexGprog f s.
+Proof.
+  intros. apply gprog_gmerge_sub; auto.
+  apply list_norepet_wrap_gprog.
+  apply list_norepet_append.
+  apply list_norepet_vprog.
+  apply G_merge_LNR.
+  apply list_norepet_spec_gprog.
+  apply list_norepet_wrap_gprog.
+  apply list_disjoint_vprog_gprog.
+Qed.
+
+Lemma gprog_spec_sub: forall f s,
+  semax_body BtreeIndexVprog spec_gprog f s ->
+  semax_body BtreeIndexVprog BtreeIndexGprog f s.
+Proof.
+  intros. unfold BtreeIndexGprog. 
+  unfold internal_specs.
+  rewrite g_merge_comm. 
+  apply gprog_gmerge_sub; auto.
+  apply list_norepet_spec_gprog.
+  apply list_norepet_append.
+  apply list_norepet_vprog.
+  apply G_merge_LNR.
+  apply list_norepet_wrap_gprog.
+  apply list_norepet_spec_gprog.
+  rewrite g_merge_comm.
+  apply list_disjoint_vprog_gprog.
+Qed.
+
+Lemma cardinality_verif:
+  semax_body BtreeIndexVprog BtreeIndexGprog f_RL_NumRecords cardinality_funspec.
+Proof.
   eapply semax_body_funspec_sub. 
-    { replace BtreeIndexVprog with btrees_sep.Vprog by auto.
-      assert (K: BtreeIndexGprog = btrees_spec.Gprog). admit. rewrite K.
-      apply body_NewCursor. }  apply sub_create_cursor.
-      simpl. repeat apply list_norepet_cons; auto; 
-      try apply list_norepet_nil. 
-      unfold not. intros. inversion H. inversion H0. 
-      inversion H0. inversion H1. inversion H1. inversion H2. inversion H2.
-      unfold not. intros. inversion H. inversion H0. inversion H0. inversion H1.
-      inversion H1. unfold not. intros. inversion H. inversion H0. inversion H0.
+  2: eapply sub_cardinality.
+  apply gprog_wrap_sub.
+  apply body_NumRecords.
+  simpl. 
+  assert (K: list_norepet [_t'1]). 
+  apply list_norepet_cons. 2: apply list_norepet_nil.
+  inversion 1. assert (M: list_norepet[_t'2; _t'1]).
+  apply list_norepet_cons; auto. inversion 1.
+  inversion H0. inversion H0.
+  apply list_norepet_cons; auto. 
+  inversion 1.
+  inversion H0. inversion H0. inversion H1. inversion H1.
+Qed.
 
-Admitted. 
-
-Lemma move_to_next_verif:
-    semax_body BtreeIndexVprog BtreeIndexGprog f_RL_MoveToNext move_to_next_funspec.
-Proof. 
-    eapply semax_body_funspec_sub. 
-    { replace BtreeIndexVprog with btrees_sep.Vprog by auto.
-      assert (K: BtreeIndexGprog = btrees_spec.Gprog). admit. rewrite K.
-      apply  } apply sub_create_index.
-      simpl. repeat apply list_norepet_cons; auto; 
-      try apply list_norepet_nil. 
-      unfold not. intros. inversion H. inversion H0. 
-      inversion H0. inversion H1. inversion H1. inversion H2. inversion H2.
-      unfold not. intros. inversion H. inversion H0. inversion H0. inversion H1.
-      inversion H1. unfold not. intros. inversion H. inversion H0. inversion H0.
-
-
-*)
-
-Lemma move_to_previous_verif:
-    semax_body BtreeIndexVprog BtreeIndexGprog f_RL_MoveToPrevious move_to_previous_funspec.
-Proof. Admitted.
-
-Lemma move_to_first_verif:
-    semax_body BtreeIndexVprog BtreeIndexGprog f_RL_MoveToFirst move_to_first_funspec.
-Proof. Admitted.
-
-Lemma go_to_key_verif:
-    semax_body BtreeIndexVprog BtreeIndexGprog f_goToKey go_to_key_funspec.
-Proof. Admitted.
-
-Lemma get_record_verif:
-    semax_body BtreeIndexVprog BtreeIndexGprog f_RL_GetRecord get_record_funspec.
-Proof. Admitted.
-
-Lemma put_record_verif:
-    semax_body BtreeIndexVprog BtreeIndexGprog f_RL_PutRecord put_record_funspec.
-Proof. Admitted.
-    
-
-
-  Definition BtreeIndexComponent: @Component NullExtension.Espec BtreeIndexVprog _ 
-      nil [] prog BI_ASI.
-  Proof. Admitted. (*
-    mkComponent internal_specs.
-   
-  + solve_SF_internal consConn_verif.
+Definition BtreeIndexComponent: @Component NullExtension.Espec BtreeIndexVprog _ 
+      nil [] prog [] [].
+Proof.
+  mkComponent. 
+  admit. admit. admit.
+  + solve_SF_internal create_index_verif.
   + solve_SF_internal newDB_verif.
   + discriminate.
-  Defined.*)
+  Defined.
+
+
+Lemma create_index_verif:
+  semax_body BtreeIndexVprog BtreeIndexGprog f_RL_NewRelation create_index_funspec.
+Proof. 
+  eapply semax_body_funspec_sub.
+  2: eapply sub_create_index.
+  apply gprog_spec_sub.
+  apply body_NewRelation.
+  simpl.
+  assert (K: list_norepet [_t'1]). 
+  apply list_norepet_cons. 2: apply list_norepet_nil.
+  inversion 1. assert (M: list_norepet[_t'2; _t'1]).
+  apply list_norepet_cons; auto. inversion 1.
+  inversion H0. inversion H0.
+  assert (N: list_norepet [_pNewRelation; _t'2; _t'1]).
+  apply list_norepet_cons; auto. 
+  inversion 1.
+  inversion H0. inversion H0. inversion H1. inversion H1.
+  apply list_norepet_cons; auto.
+  inversion 1. inversion H0. inversion H0.
+  inversion H1. inversion H1. inversion H2. inversion H2.
+Qed.
+
+
+Lemma create_cursor_verif:
+  semax_body BtreeIndexVprog BtreeIndexGprog f_RL_NewCursor create_cursor_funspec.
+Proof. 
+  eapply semax_body_funspec_sub.
+  2: eapply sub_create_cursor.
+  apply gprog_spec_sub.
+  apply body_NewCursor.
+  simpl.
+  assert (K: list_norepet [_t'2]). 
+  apply list_norepet_cons. 2: apply list_norepet_nil.
+  inversion 1. assert (M: list_norepet[_t'1; _t'2]).
+  apply list_norepet_cons; auto. inversion 1.
+  inversion H0. inversion H0.
+  assert (N: list_norepet [_i; _t'1; _t'2]).
+  apply list_norepet_cons; auto. 
+  inversion 1.
+  inversion H0. inversion H0. inversion H1. inversion H1.
+  assert (O: list_norepet [_cursor; _i; _t'1; _t'2]).
+  apply list_norepet_cons; auto. 
+  inversion 1.
+  inversion H0. inversion H0. inversion H1. inversion H1.
+  inversion H2. inversion H2.
+  apply list_norepet_cons; auto.
+  inversion 1. inversion H0. inversion H0.
+  inversion H1. inversion H1. inversion H2. inversion H2.
+  inversion H3. inversion H3.
+Qed.
+
+(*
+Lemma move_to_next_verif:
+  semax_body BtreeIndexVprog btrees_spec.Gprog f_RL_MoveToNext move_to_next_funspec.
+Proof. 
+  eapply semax_body_funspec_sub.
+  2: eapply sub_move_to_next.
+  apply body_RL_MoveToNext.
+  simpl.
+  assert (K: list_norepet [_t'3]). 
+  apply list_norepet_cons. 2: apply list_norepet_nil.
+  inversion 1. assert (M: list_norepet[_t'1; _t'3]).
+  apply list_norepet_cons; auto. inversion 1.
+  inversion H0. inversion H0.
+  assert (N: list_norepet [_t'2; _t'1; _t'3]).
+  apply list_norepet_cons; auto. 
+  inversion 1.
+  inversion H0. inversion H0. inversion H1. inversion H1.
+  apply list_norepet_cons; auto. 
+  inversion 1.
+  inversion H0. inversion H0. inversion H1. inversion H1.
+  inversion H2. inversion H2.
+Qed.
+
+Lemma move_to_previous_verif:
+    semax_body BtreeIndexVprog btrees_spec.Gprog f_RL_MoveToPrevious move_to_previous_funspec.
+Proof.
+  eapply semax_body_funspec_sub.
+  2: eapply sub_move_to_previous.
+  apply body_RL_MoveToPrevious.
+  simpl.
+  assert (K: list_norepet [_t'1]). 
+  apply list_norepet_cons. 2: apply list_norepet_nil.
+  inversion 1.
+  apply list_norepet_cons; auto. 
+  inversion 1.
+  inversion H0. inversion H0.
+Qed.
+
+Lemma move_to_first_verif:
+  semax_body BtreeIndexVprog btree_wrappers.Gprog f_RL_MoveToFirst move_to_first_funspec.
+Proof. 
+  eapply semax_body_funspec_sub.
+  2: eapply sub_move_to_first.
+  apply body_RL_MoveToFirst.
+  simpl.
+  assert (K: list_norepet [_t'2]). 
+  apply list_norepet_cons. 2: apply list_norepet_nil.
+  inversion 1. assert (M: list_norepet[_t'3; _t'2]).
+  apply list_norepet_cons; auto. inversion 1.
+  inversion H0. inversion H0.
+  assert (N: list_norepet [_t'1; _t'3; _t'2]).
+  apply list_norepet_cons; auto. 
+  inversion 1.
+  inversion H0. inversion H0. inversion H1. inversion H1.
+  apply list_norepet_cons; auto. 
+  inversion 1.
+  inversion H0. inversion H0. inversion H1. inversion H1.
+  inversion H2. inversion H2.
+Qed.
+
+
+Lemma go_to_key_verif:
+  semax_body BtreeIndexVprog btrees_spec.Gprog f_goToKey go_to_key_funspec.
+Proof.
+  eapply semax_body_funspec_sub.
+  2: eapply sub_go_to_key.
+  apply body_goToKey.
+  simpl.
+  assert (K: list_norepet [_t'2]). 
+  apply list_norepet_cons. 2: apply list_norepet_nil.
+  inversion 1. assert (M: list_norepet[_t'1; _t'2]).
+  apply list_norepet_cons; auto. inversion 1.
+  inversion H0. inversion H0.
+  assert (N: list_norepet [_key; _t'1; _t'2]).
+  apply list_norepet_cons; auto. 
+  inversion 1.
+  inversion H0. inversion H0. inversion H1. inversion H1.
+  apply list_norepet_cons; auto. 
+  inversion 1.
+  inversion H0. inversion H0. inversion H1. inversion H1.
+  inversion H2. inversion H2.
+Qed.
+
+
+Lemma get_record_verif:
+  semax_body BtreeIndexVprog btrees_spec.Gprog f_RL_GetRecord get_record_funspec.
+Proof.
+  eapply semax_body_funspec_sub.
+  2: eapply sub_get_record.
+  apply body_RL_GetRecord.
+  simpl.
+  assert (K: list_norepet [_t'6]). 
+  apply list_norepet_cons. 2: apply list_norepet_nil.
+  inversion 1. assert (M: list_norepet[_t'7; _t'6]).
+  apply list_norepet_cons; auto. inversion 1.
+  inversion H0. inversion H0.
+  assert (N: list_norepet [_t'1; _t'7; _t'6]).
+  apply list_norepet_cons; auto. 
+  inversion 1.
+  inversion H0. inversion H0. inversion H1. inversion H1.
+Admitted.
+
+Lemma put_record_verif:
+  semax_body BtreeIndexVprog btrees_spec.Gprog f_RL_PutRecord put_record_funspec.
+Proof.
+  eapply semax_body_funspec_sub.
+  2: eapply sub_put_record.
+  apply body_RL_PutRecord.
+  simpl.
+  assert (K: list_norepet [_record]). 
+  apply list_norepet_cons. 2: apply list_norepet_nil.
+  inversion 1. assert (M: list_norepet[_key; _record]).
+  apply list_norepet_cons; auto. inversion 1.
+  inversion H0. inversion H0.
+  apply list_norepet_cons; auto. 
+  inversion 1.
+  inversion H0. inversion H0. inversion H1. inversion H1.
+Qed. 
+*)
+
+
 
 End BtreeIndex_Component.
-Check BtreeIndexComponent. (*: Component [] conn_imported_specs prog C_ASI*)
-
-Definition BtreeIndexCanComp := C_to_CC BtreeIndexComponent.  
